src/3d/Batch.fsti
@@ -2,8 +2,29 @@ module Batch
 open HashingOptions
 open FStar.All
 
+val verify_fst_file
+  (out_dir: string)
+  (file: string)
+: ML unit
+
+val extract_fst_file
+  (out_dir: string)
+  (file: string)
+: ML unit
+
 val check_inplace_hashes
   (files_3d_c: list string)
+: ML unit
+
+val postprocess_c
+  (clang_format: bool)
+  (clang_format_executable: string)
+  (skip_makefiles: bool)
+  (cleanup: bool)
+  (no_everparse_h: bool)
+  (save_hashes: bool)
+  (out_dir: string)
+  (files_and_modules: list (string & string))
 : ML unit
 
 val postprocess
